Put quotations in a separate file to avoid "Top" strings

Translation/FinalTranslation.v
@@ -3,7 +3,7 @@
 From Coq Require Import Bool String List BinPos Compare_dec Omega.
 From Equations Require Import Equations DepElimDec.
 From Template Require Import Ast LiftSubst Typing Checker Template.
-From Translation Require Import SAst SLiftSubst SCommon ITyping.
+From Translation Require Import SAst SLiftSubst SCommon ITyping Quotes.
 
 Import MonadNotation.
 
@@ -42,332 +42,6 @@ Instance monad_exc : MonadExc tsl_error tsl_result :=
   }.
 
 Open Scope t_scope.
-
-(* We need to assert somewhere that we ask a Σ containing Σ-types, eq-types,
-   UIP and funext.
-   The rest will be obtained through quoting.
- *)
-
-Definition J (A : Type) (u : A) (P : forall (x : A), u = x -> Type)
-           (w : P u (@eq_refl A u)) (v : A) (p : u = v) : P v p :=
-  match p with
-  | eq_refl => w
-  end.
-
-Definition transport {T1 T2 : Type} (p : T1 = T2) (t : T1) : T2 :=
-  J Type T1 (fun X e => T1 -> X) (fun x => x) T2 p t.
-
-Axiom UIP : forall {A} {x y : A} (p q : x = y), p = q.
-Axiom funext : forall {A B} {f g : forall (x : A), B x}, (forall x, f x = g x) -> f = g.
-
-Quote Definition tEq := @eq.
-Quote Definition tRefl := @eq_refl.
-Quote Definition tJ := J.
-Quote Definition tTransport := @transport.
-Quote Definition tUip := @UIP.
-Quote Definition tFunext := @funext.
-
-Definition mkEq (A u v : term) : term :=
-  tApp tEq [ A ; u ; v ].
-
-Definition mkRefl (A u : term) : term :=
-  tApp tRefl [A ; u].
-
-Definition mkJ (A u P w v p : term) : term :=
-  tApp tJ [ A ; u ; P ; w ; v ; p ].
-
-Definition mkTransport (T1 T2 p t : term) : term :=
-  tApp tTransport [ T1 ; T2 ; p ; t ].
-
-Definition mkUip (A u v p q : term) : term :=
-  tApp tUip [ A ; u ; v ; p ; q ].
-
-Definition mkFunext (A B f g e : term) : term :=
-  tApp tFunext [ A ; B ; f ; g ; e ].
-
-Inductive heq {A} (a : A) {B} (b : B) :=
-  heqPair (p : A = B) (e : transport p a = b).
-
-Notation "A ≅ B" := (heq A B) (at level 20).
-
-Lemma heq_to_eq :
-  forall {A} {u v : A},
-    u ≅ v -> u = v.
-Proof.
-  intros A u v h.
-  destruct h as [e p].
-  assert (e = eq_refl) by (apply UIP). subst.
-  reflexivity.
-Defined.
-
-Lemma heq_refl : forall {A} (a : A), a ≅ a.
-Proof.
-  intros A a.
-  exists eq_refl.
-  reflexivity.
-Defined.
-
-Lemma heq_sym :
-  forall {A} (a : A) {B} (b : B),
-    a ≅ b -> b ≅ a.
-Proof.
-  intros A a B b h.
-  destruct h as [p e].
-  destruct p. simpl in e.
-  exists eq_refl. now symmetry.
-Defined.
-
-Lemma heq_trans :
-  forall {A} (a : A) {B} (b : B) {C} (c : C),
-    a ≅ b -> b ≅ c -> a ≅ c.
-Proof.
-  intros A a B b C c e1 e2.
-  destruct e1 as [p1 e1]. destruct e2 as [p2 e2].
-  destruct p1. destruct p2.
-  exists eq_refl. simpl in *.
-  now transitivity b.
-Defined.
-
-Lemma heq_transport :
-  forall {T T'} (p : T = T') (t : T),
-    t ≅ transport p t.
-Proof.
-  intros T T' p t.
-  exists p. reflexivity.
-Defined.
-
-Record Pack A1 A2 := pack {
-  ProjT1 : A1 ;
-  ProjT2 : A2 ;
-  ProjTe : ProjT1 ≅ ProjT2
-}.
-
-Arguments pack {_ _} _ _ _.
-Arguments ProjT1 {_ _} _.
-Arguments ProjT2 {_ _} _.
-Arguments ProjTe {_ _} _.
-
-Lemma cong_prod :
-  forall (A1 A2 : Type) (B1 : A1 -> Type) (B2 : A2 -> Type),
-    A1 ≅ A2 ->
-    (forall (p : Pack A1 A2), B1 (ProjT1 p) ≅ B2 (ProjT2 p)) ->
-    (forall x, B1 x) ≅ (forall y, B2 y).
-Proof.
-  intros A1 A2 B1 B2 hA hB.
-  exists eq_refl. simpl.
-  destruct hA as [pT pA]. rewrite (UIP pT eq_refl) in pA.
-  simpl in pA. clear pT. destruct pA. rename A1 into A.
-  assert (pB : B1 = B2).
-  { apply funext. intro x.
-    destruct (hB (pack x x (heq_refl x))) as [pT pB]. cbn in pB.
-    rewrite (UIP pT eq_refl) in pB. simpl in pB. clear pT.
-    exact pB.
-  }
-  now destruct pB.
-Defined.
-
-Lemma cong_lambda :
-  forall (A1 A2 : Type) (B1 : A1 -> Type) (B2 : A2 -> Type)
-    (f1 : forall x, B1 x) (f2 : forall x, B2 x),
-    A1 ≅ A2 ->
-    (forall (p : Pack A1 A2), B1 (ProjT1 p) ≅ B2 (ProjT2 p)) ->
-    (forall (p : Pack A1 A2), f1 (ProjT1 p) ≅ f2 (ProjT2 p)) ->
-    (fun x => f1 x) ≅ (fun x => f2 x).
-Proof.
-  intros A1 A2 B1 B2 f1 f2 pA hB hf.
-  destruct pA as [pT pA].
-  rewrite (UIP pT eq_refl) in pA. simpl in pA. clear pT.
-  destruct pA. rename A1 into A.
-  assert (pB : B1 = B2).
-  { apply funext. intro x.
-    destruct (hB (pack x x (heq_refl x))) as [pT pB].
-    rewrite (UIP pT eq_refl) in pB. simpl in pB. clear pT.
-    exact pB.
-  }
-  destruct pB. rename B1 into B. clear hB.
-  exists eq_refl. simpl.
-  apply funext. intro x.
-  destruct (hf (pack x x (heq_refl x))) as [p pf].
-  now rewrite (UIP p eq_refl) in pf.
-Defined.
-
-Lemma cong_app :
-  forall (A1 A2 : Type) (B1 : A1 -> Type) (B2 : A2 -> Type)
-    (f1 : forall x, B1 x) (f2 : forall x, B2 x)
-    (u1 : A1) (u2 : A2),
-    A1 ≅ A2 ->
-    (forall (p : Pack A1 A2), B1 (ProjT1 p) ≅ B2 (ProjT2 p)) ->
-    f1 ≅ f2 ->
-    u1 ≅ u2 ->
-    f1 u1 ≅ f2 u2.
-Proof.
-  intros A1 A2 B1 B2 f1 f2 u1 u2 pA hB pf pu.
-  destruct pA as [pT pA].
-  rewrite (UIP pT eq_refl) in pA. simpl in pA. clear pT.
-  destruct pA. rename A1 into A.
-  assert (pB : B1 = B2).
-  { apply funext. intro x.
-    destruct (hB (pack x x (heq_refl x))) as [pT pB].
-    rewrite (UIP pT eq_refl) in pB. simpl in pB. clear pT.
-    exact pB.
-  }
-  destruct pB. rename B1 into B. clear hB.
-  destruct pf as [p pf].
-  rewrite (UIP p eq_refl) in pf. simpl in pf. clear p.
-  destruct pf. rename f1 into f.
-  destruct pu as [p pu].
-  rewrite (UIP p eq_refl) in pu. simpl in pu. clear p.
-  destruct pu. rename u1 into u.
-  now apply heq_refl.
-Defined.
-
-Lemma cong_eq :
-  forall (A1 A2 : Type) (u1 v1 : A1) (u2 v2 : A2),
-    A1 ≅ A2 -> u1 ≅ u2 -> v1 ≅ v2 -> (u1 = v1) ≅ (u2 = v2).
-Proof.
-  intros A1 A2 u1 v1 u2 v2 pA pu pv.
-  destruct pA as [pT pA].
-  rewrite (UIP pT eq_refl) in pA. simpl in pA. clear pT.
-  destruct pA. rename A1 into A.
-  destruct pu as [pA pu].
-  rewrite (UIP pA eq_refl) in pu. simpl in pu. clear pA.
-  destruct pu. rename u1 into u.
-  destruct pv as [pA pv].
-  rewrite (UIP pA eq_refl) in pv. simpl in pv. clear pA.
-  destruct pv. rename v1 into v.
-  apply heq_refl.
-Defined.
-
-Lemma cong_refl :
-  forall (A1 A2 : Type) (u1 : A1) (u2 : A2),
-    A1 ≅ A2 ->
-    u1 ≅ u2 ->
-    @eq_refl A1 u1 ≅ @eq_refl A2 u2.
-Proof.
-  intros A1 A2 u1 u2 pA pu.
-  destruct pA as [pT pA].
-  rewrite (UIP pT eq_refl) in pA. simpl in pA. clear pT.
-  destruct pA. rename A1 into A.
-  destruct pu as [pA pu].
-  rewrite (UIP pA eq_refl) in pu. simpl in pu. clear pA.
-  destruct pu.
-  now apply heq_refl.
-Defined.
-
-Lemma eq_to_heq :
-  forall {A} {u v : A},
-    u = v -> u ≅ v.
-Proof.
-  intros A u v p.
-  exists eq_refl. exact p.
-Defined.
-
-Lemma heq_type_eq :
-  forall {A} {u : A} {B} {v : B},
-    u ≅ v -> A = B.
-Proof.
-  intros A u B v e.
-  now destruct e.
-Defined.
-
-Quote Definition tHeq := @heq.
-Quote Definition tHeqToEq := @heq_to_eq.
-Quote Definition tHeqRefl := @heq_refl.
-Quote Definition tHeqSym := @heq_sym.
-Quote Definition tHeqTrans := @heq_trans.
-Quote Definition tHeqTransport := @heq_transport.
-Quote Definition tPack := @Pack.
-Quote Definition tProjT1 := @ProjT1.
-Quote Definition tProjT2 := @ProjT2.
-Quote Definition tProjTe := @ProjTe.
-Quote Definition tCongProd := @cong_prod.
-Quote Definition tCongLambda := @cong_lambda.
-Quote Definition tCongApp := @cong_app.
-Quote Definition tCongEq := @cong_eq.
-Quote Definition tCongRefl := @cong_refl.
-Quote Definition tEqToHeq := @eq_to_heq.
-Quote Definition tHeqTypeEq := @heq_type_eq.
-
-Definition mkHeq (A a B b : term) : term :=
-  tApp tHeq [ A ; a ; B ; b ].
-
-Definition mkHeqToHeq (A u v p : term) : term :=
-  tApp tHeqToEq [ A ; u ; v ; p ].
-
-Definition mkHeqRefl (A a : term) : term :=
-  tApp tHeqRefl [ A ; a ].
-
-Definition mkHeqSym (A a B b p : term) : term :=
-  tApp tHeqSym [ A ; a ; B ; b ; p ].
-
-Definition mkHeqTrans (A a B b C c p q : term) : term :=
-  tApp tHeqTrans [ A ; a ; B ; b ; C ; c ; p ; q ].
-
-Definition mkHeqTransport (A B p t : term) : term :=
-  tApp tHeqTransport [ A ; B ; p ; t ].
-
-Definition mkPack (A1 A2 : term) : term :=
-  tApp tPack [ A1 ; A2 ].
-
-Definition mkProjT1 (A1 A2 p : term) : term :=
-  tApp tProjT1 [ A1 ; A2 ; p ].
-
-Definition mkProjT2 (A1 A2 p : term) : term :=
-  tApp tProjT2 [ A1 ; A2 ; p ].
-
-Definition mkProjTe (A1 A2 p : term) : term :=
-  tApp tProjTe [ A1 ; A2 ; p ].
-
-Definition mkCongProd (A1 A2 B1 B2 pA pB : term) :=
-  tApp tCongProd [
-    A1 ;
-    A2 ;
-    (tLambda nAnon A1 B1) ;
-    (tLambda nAnon A2 B2) ;
-    pA ;
-    (tLambda nAnon (mkPack A1 A2) pB)
-  ].
-
-Definition mkCongLambda (A1 A2 B1 B2 t1 t2 pA pB pt : term) :=
-  tApp tCongProd [
-    A1 ;
-    A2 ;
-    (tLambda nAnon A1 B1) ;
-    (tLambda nAnon A2 B2) ;
-    (tLambda nAnon A1 t1) ;
-    (tLambda nAnon A2 t2) ;
-    pA ;
-    (tLambda nAnon (mkPack A1 A2) pB) ;
-    (tLambda nAnon (mkPack A1 A2) pt)
-  ].
-
-Definition mkCongApp (A1 A2 B1 B2 t1 t2 u1 u2 pA pB pt pu : term) :=
-  tApp tCongProd [
-    A1 ;
-    A2 ;
-    (tLambda nAnon A1 B1) ;
-    (tLambda nAnon A2 B2) ;
-    t1 ;
-    t2 ;
-    u1 ;
-    u2 ;
-    pA ;
-    (tLambda nAnon (mkPack A1 A2) pB) ;
-    pt ;
-    pu
-  ].
-
-Definition mkCongEq (A1 A2 u1 v1 u2 v2 pA pu pv : term) : term :=
-  tApp tCongEq [ A1 ; A2 ; u1 ; v1 ; u2 ; v2 ; pA ; pu ; pv ].
-
-Definition mkCongRefl (A1 A2 u1 u2 pA pu : term) : term :=
-  tApp tCongRefl [ A1 ; A2 ; u1 ; u2 ; pA ; pu ].
-
-Definition mkEqToHeq (A u v p : term) : term :=
-  tApp tEqToHeq [ A ; u ; v ; p ].
-
-Definition mkHeqTypeEq (A u B v p : term) : term :=
-  tApp tHeqTypeEq [ A ; u ; B ; v ; p ].
 
 Fixpoint tsl_rec (fuel : nat) (Σ : global_context) (Γ : context) (t : sterm) {struct fuel}
   : tsl_result term :=
@@ -421,7 +95,7 @@ Fixpoint tsl_rec (fuel : nat) (Σ : global_context) (Γ : context) (t : sterm) {
     | sHeqToEq p =>
       p' <- tsl_rec fuel Σ Γ p ;;
       match @infer (Build_Fuel fuel) Σ Γ p' with
-      | Checked (tApp (tInd (mkInd "Top.heq" 0) _) [ A' ; u' ; _ ; v' ]) =>
+      | Checked (tApp (tInd (mkInd "Translation.Quotes.heq" 0) _) [ A' ; u' ; _ ; v' ]) =>
         ret (mkHeqToHeq A' u' v' p')
       (* That's not really the correct error but well. *)
       | Checked T => raise (TypingError (NotAnInductive T))
@@ -434,7 +108,7 @@ Fixpoint tsl_rec (fuel : nat) (Σ : global_context) (Γ : context) (t : sterm) {
     | sHeqSym p =>
       p' <- tsl_rec fuel Σ Γ p ;;
       match @infer (Build_Fuel fuel) Σ Γ p' with
-      | Checked (tApp (tInd (mkInd "Top.heq" 0) _) [ A' ; a' ; B' ; b' ]) =>
+      | Checked (tApp (tInd (mkInd "Translation.Quotes.heq" 0) _) [ A' ; a' ; B' ; b' ]) =>
         ret (mkHeqSym A' a' B' b' p')
       | Checked T => raise (TypingError (NotAnInductive T))
       | TypeError t => raise (TypingError t)
@@ -443,9 +117,9 @@ Fixpoint tsl_rec (fuel : nat) (Σ : global_context) (Γ : context) (t : sterm) {
       p' <- tsl_rec fuel Σ Γ p ;;
       q' <- tsl_rec fuel Σ Γ q ;;
       match @infer (Build_Fuel fuel) Σ Γ p' with
-      | Checked (tApp (tInd (mkInd "Top.heq" 0) _) [ A' ; a' ; B' ; b' ]) =>
+      | Checked (tApp (tInd (mkInd "Translation.Quotes.heq" 0) _) [ A' ; a' ; B' ; b' ]) =>
         match @infer (Build_Fuel fuel) Σ Γ q' with
-        | Checked (tApp (tInd (mkInd "Top.heq" 0) _) [ _ ; _ ; C' ; c' ]) =>
+        | Checked (tApp (tInd (mkInd "Translation.Quotes.heq" 0) _) [ _ ; _ ; C' ; c' ]) =>
           ret (mkHeqTrans A' a' B' b' C' c' p' q')
         | Checked T => raise (TypingError (NotAnInductive T))
         | TypeError t => raise (TypingError t)
@@ -465,7 +139,7 @@ Fixpoint tsl_rec (fuel : nat) (Σ : global_context) (Γ : context) (t : sterm) {
     | sCongProd B1 B2 pA pB =>
       pA' <- tsl_rec fuel Σ Γ pA ;;
       match @infer (Build_Fuel fuel) Σ Γ pA' with
-      | Checked (tApp (tInd (mkInd "Top.heq" 0) _) [ _ ; A1' ; _ ; A2' ]) =>
+      | Checked (tApp (tInd (mkInd "Translation.Quotes.heq" 0) _) [ _ ; A1' ; _ ; A2' ]) =>
         pB' <- tsl_rec fuel Σ (Γ ,, vass nAnon (mkPack A1' A2')) pB ;;
         B1' <- tsl_rec fuel Σ (Γ ,, vass nAnon A1') B1 ;;
         B2' <- tsl_rec fuel Σ (Γ ,, vass nAnon A2') B2 ;;
@@ -476,7 +150,7 @@ Fixpoint tsl_rec (fuel : nat) (Σ : global_context) (Γ : context) (t : sterm) {
     | sCongLambda B1 B2 t1 t2 pA pB pt =>
       pA' <- tsl_rec fuel Σ Γ pA ;;
       match @infer (Build_Fuel fuel) Σ Γ pA' with
-      | Checked (tApp (tInd (mkInd "Top.heq" 0) _) [ _ ; A1' ; _ ; A2' ]) =>
+      | Checked (tApp (tInd (mkInd "Translation.Quotes.heq" 0) _) [ _ ; A1' ; _ ; A2' ]) =>
         pB' <- tsl_rec fuel Σ (Γ ,, vass nAnon (mkPack A1' A2')) pB ;;
         pt' <- tsl_rec fuel Σ (Γ ,, vass nAnon (mkPack A1' A2')) pt ;;
         B1' <- tsl_rec fuel Σ (Γ ,, vass nAnon A1') B1 ;;
@@ -490,16 +164,16 @@ Fixpoint tsl_rec (fuel : nat) (Σ : global_context) (Γ : context) (t : sterm) {
     | sCongApp B1 B2 pt pA pB pu =>
       pA' <- tsl_rec fuel Σ Γ pA ;;
       match @infer (Build_Fuel fuel) Σ Γ pA' with
-      | Checked (tApp (tInd (mkInd "Top.heq" 0) _) [ _ ; A1' ; _ ; A2' ]) =>
+      | Checked (tApp (tInd (mkInd "Translation.Quotes.heq" 0) _) [ _ ; A1' ; _ ; A2' ]) =>
         pB' <- tsl_rec fuel Σ (Γ ,, vass nAnon (mkPack A1' A2')) pB ;;
         pt' <- tsl_rec fuel Σ Γ pt ;;
         pu' <- tsl_rec fuel Σ Γ pu ;;
         B1' <- tsl_rec fuel Σ (Γ ,, vass nAnon A1') B1 ;;
         B2' <- tsl_rec fuel Σ (Γ ,, vass nAnon A2') B2 ;;
         match @infer (Build_Fuel fuel) Σ Γ pt' with
-        | Checked (tApp (tInd (mkInd "Top.heq" 0) _) [ _ ; t1' ; _ ; t2' ]) =>
+        | Checked (tApp (tInd (mkInd "Translation.Quotes.heq" 0) _) [ _ ; t1' ; _ ; t2' ]) =>
           match @infer (Build_Fuel fuel) Σ Γ pt' with
-          | Checked (tApp (tInd (mkInd "Top.heq" 0) _) [ _ ; u1' ; _ ; u2' ]) =>
+          | Checked (tApp (tInd (mkInd "Translation.Quotes.heq" 0) _) [ _ ; u1' ; _ ; u2' ]) =>
             ret (mkCongApp A1' A2' B1' B2' t1' t2' u1' u2' pA' pB' pt' pu')
           | Checked T => raise (TypingError (NotAnInductive T))
           | TypeError t => raise (TypingError t)
@@ -515,9 +189,9 @@ Fixpoint tsl_rec (fuel : nat) (Σ : global_context) (Γ : context) (t : sterm) {
       pu' <- tsl_rec fuel Σ Γ pu ;;
       pv' <- tsl_rec fuel Σ Γ pv ;;
       match @infer (Build_Fuel fuel) Σ Γ pu' with
-      | Checked (tApp (tInd (mkInd "Top.heq" 0) _) [ A1' ; u1' ; A2' ; u2' ]) =>
+      | Checked (tApp (tInd (mkInd "Translation.Quotes.heq" 0) _) [ A1' ; u1' ; A2' ; u2' ]) =>
         match @infer (Build_Fuel fuel) Σ Γ pv' with
-        | Checked (tApp (tInd (mkInd "Top.heq" 0) _) [ _ ; v1' ; _ ; v2' ]) =>
+        | Checked (tApp (tInd (mkInd "Translation.Quotes.heq" 0) _) [ _ ; v1' ; _ ; v2' ]) =>
           ret (mkCongEq A1' A2' u1' v1' u2' v2' pA' pu' pv')
         | Checked T => raise (TypingError (NotAnInductive T))
         | TypeError t => raise (TypingError t)
@@ -529,7 +203,7 @@ Fixpoint tsl_rec (fuel : nat) (Σ : global_context) (Γ : context) (t : sterm) {
       pA' <- tsl_rec fuel Σ Γ pA ;;
       pu' <- tsl_rec fuel Σ Γ pu ;;
       match @infer (Build_Fuel fuel) Σ Γ pu' with
-      | Checked (tApp (tInd (mkInd "Top.heq" 0) _) [ A1' ; u1' ; A2' ; u2' ]) =>
+      | Checked (tApp (tInd (mkInd "Translation.Quotes.heq" 0) _) [ A1' ; u1' ; A2' ; u2' ]) =>
         ret (mkCongRefl A1' A2' u1' u2' pA' pu')
       | Checked T => raise (TypingError (NotAnInductive T))
       | TypeError t => raise (TypingError t)
@@ -545,7 +219,7 @@ Fixpoint tsl_rec (fuel : nat) (Σ : global_context) (Γ : context) (t : sterm) {
     | sHeqTypeEq p =>
       p' <- tsl_rec fuel Σ Γ p ;;
       match @infer (Build_Fuel fuel) Σ Γ p' with
-      | Checked (tApp (tInd (mkInd "Top.heq" 0) _) [ A' ; u' ; B' ; v' ]) =>
+      | Checked (tApp (tInd (mkInd "Translation.Quotes.heq" 0) _) [ A' ; u' ; B' ; v' ]) =>
         ret (mkHeqTypeEq A' u' B' v' p')
       | Checked T => raise (TypingError (NotAnInductive T))
       | TypeError t => raise (TypingError t)
@@ -557,7 +231,7 @@ Fixpoint tsl_rec (fuel : nat) (Σ : global_context) (Γ : context) (t : sterm) {
     | sProjT1 p =>
       p' <- tsl_rec fuel Σ Γ p ;;
       match @infer (Build_Fuel fuel) Σ Γ p' with
-      | Checked (tApp (tInd (mkInd "Top.Pack" 0) _) [ A1' ; A2' ]) =>
+      | Checked (tApp (tInd (mkInd "Translation.Quotes.Pack" 0) _) [ A1' ; A2' ]) =>
         ret (mkProjT1 A1' A2' p')
       | Checked T => raise (TypingError (NotAnInductive T))
       | TypeError t => raise (TypingError t)
@@ -565,7 +239,7 @@ Fixpoint tsl_rec (fuel : nat) (Σ : global_context) (Γ : context) (t : sterm) {
     | sProjT2 p =>
       p' <- tsl_rec fuel Σ Γ p ;;
       match @infer (Build_Fuel fuel) Σ Γ p' with
-      | Checked (tApp (tInd (mkInd "Top.Pack" 0) _) [ A1' ; A2' ]) =>
+      | Checked (tApp (tInd (mkInd "Translation.Quotes.Pack" 0) _) [ A1' ; A2' ]) =>
         ret (mkProjT2 A1' A2' p')
       | Checked T => raise (TypingError (NotAnInductive T))
       | TypeError t => raise (TypingError t)
@@ -573,7 +247,7 @@ Fixpoint tsl_rec (fuel : nat) (Σ : global_context) (Γ : context) (t : sterm) {
     | sProjTe p =>
       p' <- tsl_rec fuel Σ Γ p ;;
       match @infer (Build_Fuel fuel) Σ Γ p' with
-      | Checked (tApp (tInd (mkInd "Top.Pack" 0) _) [ A1' ; A2' ]) =>
+      | Checked (tApp (tInd (mkInd "Translation.Quotes.Pack" 0) _) [ A1' ; A2' ]) =>
         ret (mkProjTe A1' A2' p')
       | Checked T => raise (TypingError (NotAnInductive T))
       | TypeError t => raise (TypingError t)
@@ -650,111 +324,111 @@ Definition eq_decl :=
 
 Quote Recursively Definition J_prog := J.
 Definition J_decl :=
-  Eval compute in (get_cdecl "Top.J" J_prog).
+  Eval compute in (get_cdecl "Translation.Quotes.J" J_prog).
 
 Quote Recursively Definition Transport_prog := @transport.
 Definition Transport_decl :=
-  Eval compute in (get_cdecl "Top.transport" Transport_prog).
+  Eval compute in (get_cdecl "Translation.Quotes.transport" Transport_prog).
 
 Quote Recursively Definition UIP_prog := @UIP.
 Definition UIP_decl :=
-  Eval compute in (get_adecl "Top.UIP" UIP_prog).
+  Eval compute in (get_adecl "Translation.Quotes.UIP" UIP_prog).
 
 Quote Recursively Definition funext_prog := @funext.
 Definition funext_decl :=
-  Eval compute in (get_adecl "Top.funext" funext_prog).
+  Eval compute in (get_adecl "Translation.Quotes.funext" funext_prog).
 
 Quote Recursively Definition heq_prog := @heq.
 Definition heq_decl :=
-  Eval compute in (get_idecl "Top.heq" heq_prog).
+  Eval compute in (get_idecl "Translation.Quotes.heq" heq_prog).
 
 Quote Recursively Definition heq_to_eq_prog := @heq_to_eq.
 Definition heq_to_eq_decl :=
-  Eval compute in (get_cdecl "Top.heq_to_eq" heq_to_eq_prog).
+  Eval compute in (get_cdecl "Translation.Quotes.heq_to_eq" heq_to_eq_prog).
 
 Quote Recursively Definition heq_refl_prog := @heq_refl.
 Definition heq_refl_decl :=
-  Eval compute in (get_cdecl "Top.heq_refl" heq_refl_prog).
+  Eval compute in (get_cdecl "Translation.Quotes.heq_refl" heq_refl_prog).
 
 Quote Recursively Definition heq_sym_prog := @heq_sym.
 Definition heq_sym_decl :=
-  Eval compute in (get_cdecl "Top.heq_sym" heq_sym_prog).
+  Eval compute in (get_cdecl "Translation.Quotes.heq_sym" heq_sym_prog).
 
 Quote Recursively Definition heq_trans_prog := @heq_trans.
 Definition heq_trans_decl :=
-  Eval compute in (get_cdecl "Top.heq_trans" heq_trans_prog).
+  Eval compute in (get_cdecl "Translation.Quotes.heq_trans" heq_trans_prog).
 
 Quote Recursively Definition heq_transport_prog := @heq_transport.
 Definition heq_transport_decl :=
-  Eval compute in (get_cdecl "Top.heq_transport" heq_transport_prog).
+  Eval compute in (get_cdecl "Translation.Quotes.heq_transport" heq_transport_prog).
 
 Quote Recursively Definition Pack_prog := @Pack.
 Definition Pack_decl :=
-  Eval compute in (get_idecl "Top.Pack" Pack_prog).
+  Eval compute in (get_idecl "Translation.Quotes.Pack" Pack_prog).
 
 Quote Recursively Definition ProjT1_prog := @ProjT1.
 Definition ProjT1_decl :=
-  Eval compute in (get_cdecl "Top.ProjT1" ProjT1_prog).
+  Eval compute in (get_cdecl "Translation.Quotes.ProjT1" ProjT1_prog).
 
 Quote Recursively Definition ProjT2_prog := @ProjT2.
 Definition ProjT2_decl :=
-  Eval compute in (get_cdecl "Top.ProjT2" ProjT2_prog).
+  Eval compute in (get_cdecl "Translation.Quotes.ProjT2" ProjT2_prog).
 
 Quote Recursively Definition ProjTe_prog := @ProjTe.
 Definition ProjTe_decl :=
-  Eval compute in (get_cdecl "Top.ProjTe" ProjTe_prog).
+  Eval compute in (get_cdecl "Translation.Quotes.ProjTe" ProjTe_prog).
 
 Quote Recursively Definition cong_prod_prog := @cong_prod.
 Definition cong_prod_decl :=
-  Eval compute in (get_cdecl "Top.cong_prod" cong_prod_prog).
+  Eval compute in (get_cdecl "Translation.Quotes.cong_prod" cong_prod_prog).
 
 Quote Recursively Definition cong_lambda_prog := @cong_lambda.
 Definition cong_lambda_decl :=
-  Eval compute in (get_cdecl "Top.cong_lambda" cong_lambda_prog).
+  Eval compute in (get_cdecl "Translation.Quotes.cong_lambda" cong_lambda_prog).
 
 Quote Recursively Definition cong_app_prog := @cong_app.
 Definition cong_app_decl :=
-  Eval compute in (get_cdecl "Top.cong_app" cong_app_prog).
+  Eval compute in (get_cdecl "Translation.Quotes.cong_app" cong_app_prog).
 
 Quote Recursively Definition cong_eq_prog := @cong_eq.
 Definition cong_eq_decl :=
-  Eval compute in (get_cdecl "Top.cong_eq" cong_eq_prog).
+  Eval compute in (get_cdecl "Translation.Quotes.cong_eq" cong_eq_prog).
 
 Quote Recursively Definition cong_refl_prog := @cong_refl.
 Definition cong_refl_decl :=
-  Eval compute in (get_cdecl "Top.cong_refl" cong_refl_prog).
+  Eval compute in (get_cdecl "Translation.Quotes.cong_refl" cong_refl_prog).
 
 Quote Recursively Definition eq_to_heq_prog := @eq_to_heq.
 Definition eq_to_heq_decl :=
-  Eval compute in (get_cdecl "Top.eq_to_heq" eq_to_heq_prog).
+  Eval compute in (get_cdecl "Translation.Quotes.eq_to_heq" eq_to_heq_prog).
 
 Quote Recursively Definition heq_type_eq_prog := @heq_type_eq.
 Definition heq_type_eq_decl :=
-  Eval compute in (get_cdecl "Top.heq_type_eq" heq_type_eq_prog).
+  Eval compute in (get_cdecl "Translation.Quotes.heq_type_eq" heq_type_eq_prog).
 
 Definition Σ : global_context :=
   [ InductiveDecl "Coq.Init.Logic.eq" eq_decl ;
-    ConstantDecl "Top.J" J_decl ;
-    ConstantDecl "Top.transport" Transport_decl ;
-    ConstantDecl "Top.UIP" UIP_decl ;
-    ConstantDecl "Top.funext" funext_decl ;
-    InductiveDecl "Top.heq" heq_decl ;
-    ConstantDecl "Top.heq_to_eq" heq_to_eq_decl ;
-    ConstantDecl "Top.heq_refl" heq_refl_decl ;
-    ConstantDecl "Top.heq_sym" heq_sym_decl ;
-    ConstantDecl "Top.heq_trans" heq_trans_decl ;
-    ConstantDecl "Top.heq_transport" heq_transport_decl ;
-    InductiveDecl "Top.Pack" Pack_decl ;
-    ConstantDecl "Top.ProjT1" ProjT1_decl ;
-    ConstantDecl "Top.ProjT2" ProjT2_decl ;
-    ConstantDecl "Top.ProjTe" ProjTe_decl ;
-    ConstantDecl "Top.cong_prod" cong_prod_decl ;
-    ConstantDecl "Top.cong_lambda" cong_lambda_decl ;
-    ConstantDecl "Top.cong_app" cong_app_decl ;
-    ConstantDecl "Top.cong_eq" cong_eq_decl ;
-    ConstantDecl "Top.cong_refl" cong_refl_decl ;
-    ConstantDecl "Top.eq_to_heq" eq_to_heq_decl ;
-    ConstantDecl "Top.heq_type_eq" heq_type_eq_decl
+    ConstantDecl "Translation.Quotes.J" J_decl ;
+    ConstantDecl "Translation.Quotes.transport" Transport_decl ;
+    ConstantDecl "Translation.Quotes.UIP" UIP_decl ;
+    ConstantDecl "Translation.Quotes.funext" funext_decl ;
+    InductiveDecl "Translation.Quotes.heq" heq_decl ;
+    ConstantDecl "Translation.Quotes.heq_to_eq" heq_to_eq_decl ;
+    ConstantDecl "Translation.Quotes.heq_refl" heq_refl_decl ;
+    ConstantDecl "Translation.Quotes.heq_sym" heq_sym_decl ;
+    ConstantDecl "Translation.Quotes.heq_trans" heq_trans_decl ;
+    ConstantDecl "Translation.Quotes.heq_transport" heq_transport_decl ;
+    InductiveDecl "Translation.Quotes.Pack" Pack_decl ;
+    ConstantDecl "Translation.Quotes.ProjT1" ProjT1_decl ;
+    ConstantDecl "Translation.Quotes.ProjT2" ProjT2_decl ;
+    ConstantDecl "Translation.Quotes.ProjTe" ProjTe_decl ;
+    ConstantDecl "Translation.Quotes.cong_prod" cong_prod_decl ;
+    ConstantDecl "Translation.Quotes.cong_lambda" cong_lambda_decl ;
+    ConstantDecl "Translation.Quotes.cong_app" cong_app_decl ;
+    ConstantDecl "Translation.Quotes.cong_eq" cong_eq_decl ;
+    ConstantDecl "Translation.Quotes.cong_refl" cong_refl_decl ;
+    ConstantDecl "Translation.Quotes.eq_to_heq" eq_to_heq_decl ;
+    ConstantDecl "Translation.Quotes.heq_type_eq" heq_type_eq_decl
   ].
 
 (* Checking for the sake of checking *)
