Translation/Quotes.v
@@ -1,0 +1,327 @@
+(* Quotations of terms *)
+
+From Coq Require Import Bool String List BinPos Compare_dec Omega.
+From Equations Require Import Equations DepElimDec.
+From Template Require Import Ast LiftSubst Typing Checker Template.
+(* From Translation Require Import SAst SLiftSubst SCommon ITyping. *)
+
+Definition J (A : Type) (u : A) (P : forall (x : A), u = x -> Type)
+           (w : P u (@eq_refl A u)) (v : A) (p : u = v) : P v p :=
+  match p with
+  | eq_refl => w
+  end.
+
+Definition transport {T1 T2 : Type} (p : T1 = T2) (t : T1) : T2 :=
+  J Type T1 (fun X e => T1 -> X) (fun x => x) T2 p t.
+
+Axiom UIP : forall {A} {x y : A} (p q : x = y), p = q.
+Axiom funext : forall {A B} {f g : forall (x : A), B x}, (forall x, f x = g x) -> f = g.
+
+Quote Definition tEq := @eq.
+Quote Definition tRefl := @eq_refl.
+Quote Definition tJ := J.
+Quote Definition tTransport := @transport.
+Quote Definition tUip := @UIP.
+Quote Definition tFunext := @funext.
+
+Definition mkEq (A u v : term) : term :=
+  tApp tEq [ A ; u ; v ].
+
+Definition mkRefl (A u : term) : term :=
+  tApp tRefl [A ; u].
+
+Definition mkJ (A u P w v p : term) : term :=
+  tApp tJ [ A ; u ; P ; w ; v ; p ].
+
+Definition mkTransport (T1 T2 p t : term) : term :=
+  tApp tTransport [ T1 ; T2 ; p ; t ].
+
+Definition mkUip (A u v p q : term) : term :=
+  tApp tUip [ A ; u ; v ; p ; q ].
+
+Definition mkFunext (A B f g e : term) : term :=
+  tApp tFunext [ A ; B ; f ; g ; e ].
+
+Inductive heq {A} (a : A) {B} (b : B) :=
+  heqPair (p : A = B) (e : transport p a = b).
+
+Notation "A ≅ B" := (heq A B) (at level 20).
+
+Lemma heq_to_eq :
+  forall {A} {u v : A},
+    u ≅ v -> u = v.
+Proof.
+  intros A u v h.
+  destruct h as [e p].
+  assert (e = eq_refl) by (apply UIP). subst.
+  reflexivity.
+Defined.
+
+Lemma heq_refl : forall {A} (a : A), a ≅ a.
+Proof.
+  intros A a.
+  exists eq_refl.
+  reflexivity.
+Defined.
+
+Lemma heq_sym :
+  forall {A} (a : A) {B} (b : B),
+    a ≅ b -> b ≅ a.
+Proof.
+  intros A a B b h.
+  destruct h as [p e].
+  destruct p. simpl in e.
+  exists eq_refl. now symmetry.
+Defined.
+
+Lemma heq_trans :
+  forall {A} (a : A) {B} (b : B) {C} (c : C),
+    a ≅ b -> b ≅ c -> a ≅ c.
+Proof.
+  intros A a B b C c e1 e2.
+  destruct e1 as [p1 e1]. destruct e2 as [p2 e2].
+  destruct p1. destruct p2.
+  exists eq_refl. simpl in *.
+  now transitivity b.
+Defined.
+
+Lemma heq_transport :
+  forall {T T'} (p : T = T') (t : T),
+    t ≅ transport p t.
+Proof.
+  intros T T' p t.
+  exists p. reflexivity.
+Defined.
+
+Record Pack A1 A2 := pack {
+  ProjT1 : A1 ;
+  ProjT2 : A2 ;
+  ProjTe : ProjT1 ≅ ProjT2
+}.
+
+Arguments pack {_ _} _ _ _.
+Arguments ProjT1 {_ _} _.
+Arguments ProjT2 {_ _} _.
+Arguments ProjTe {_ _} _.
+
+Lemma cong_prod :
+  forall (A1 A2 : Type) (B1 : A1 -> Type) (B2 : A2 -> Type),
+    A1 ≅ A2 ->
+    (forall (p : Pack A1 A2), B1 (ProjT1 p) ≅ B2 (ProjT2 p)) ->
+    (forall x, B1 x) ≅ (forall y, B2 y).
+Proof.
+  intros A1 A2 B1 B2 hA hB.
+  exists eq_refl. simpl.
+  destruct hA as [pT pA]. rewrite (UIP pT eq_refl) in pA.
+  simpl in pA. clear pT. destruct pA. rename A1 into A.
+  assert (pB : B1 = B2).
+  { apply funext. intro x.
+    destruct (hB (pack x x (heq_refl x))) as [pT pB]. cbn in pB.
+    rewrite (UIP pT eq_refl) in pB. simpl in pB. clear pT.
+    exact pB.
+  }
+  now destruct pB.
+Defined.
+
+Lemma cong_lambda :
+  forall (A1 A2 : Type) (B1 : A1 -> Type) (B2 : A2 -> Type)
+    (f1 : forall x, B1 x) (f2 : forall x, B2 x),
+    A1 ≅ A2 ->
+    (forall (p : Pack A1 A2), B1 (ProjT1 p) ≅ B2 (ProjT2 p)) ->
+    (forall (p : Pack A1 A2), f1 (ProjT1 p) ≅ f2 (ProjT2 p)) ->
+    (fun x => f1 x) ≅ (fun x => f2 x).
+Proof.
+  intros A1 A2 B1 B2 f1 f2 pA hB hf.
+  destruct pA as [pT pA].
+  rewrite (UIP pT eq_refl) in pA. simpl in pA. clear pT.
+  destruct pA. rename A1 into A.
+  assert (pB : B1 = B2).
+  { apply funext. intro x.
+    destruct (hB (pack x x (heq_refl x))) as [pT pB].
+    rewrite (UIP pT eq_refl) in pB. simpl in pB. clear pT.
+    exact pB.
+  }
+  destruct pB. rename B1 into B. clear hB.
+  exists eq_refl. simpl.
+  apply funext. intro x.
+  destruct (hf (pack x x (heq_refl x))) as [p pf].
+  now rewrite (UIP p eq_refl) in pf.
+Defined.
+
+Lemma cong_app :
+  forall (A1 A2 : Type) (B1 : A1 -> Type) (B2 : A2 -> Type)
+    (f1 : forall x, B1 x) (f2 : forall x, B2 x)
+    (u1 : A1) (u2 : A2),
+    A1 ≅ A2 ->
+    (forall (p : Pack A1 A2), B1 (ProjT1 p) ≅ B2 (ProjT2 p)) ->
+    f1 ≅ f2 ->
+    u1 ≅ u2 ->
+    f1 u1 ≅ f2 u2.
+Proof.
+  intros A1 A2 B1 B2 f1 f2 u1 u2 pA hB pf pu.
+  destruct pA as [pT pA].
+  rewrite (UIP pT eq_refl) in pA. simpl in pA. clear pT.
+  destruct pA. rename A1 into A.
+  assert (pB : B1 = B2).
+  { apply funext. intro x.
+    destruct (hB (pack x x (heq_refl x))) as [pT pB].
+    rewrite (UIP pT eq_refl) in pB. simpl in pB. clear pT.
+    exact pB.
+  }
+  destruct pB. rename B1 into B. clear hB.
+  destruct pf as [p pf].
+  rewrite (UIP p eq_refl) in pf. simpl in pf. clear p.
+  destruct pf. rename f1 into f.
+  destruct pu as [p pu].
+  rewrite (UIP p eq_refl) in pu. simpl in pu. clear p.
+  destruct pu. rename u1 into u.
+  now apply heq_refl.
+Defined.
+
+Lemma cong_eq :
+  forall (A1 A2 : Type) (u1 v1 : A1) (u2 v2 : A2),
+    A1 ≅ A2 -> u1 ≅ u2 -> v1 ≅ v2 -> (u1 = v1) ≅ (u2 = v2).
+Proof.
+  intros A1 A2 u1 v1 u2 v2 pA pu pv.
+  destruct pA as [pT pA].
+  rewrite (UIP pT eq_refl) in pA. simpl in pA. clear pT.
+  destruct pA. rename A1 into A.
+  destruct pu as [pA pu].
+  rewrite (UIP pA eq_refl) in pu. simpl in pu. clear pA.
+  destruct pu. rename u1 into u.
+  destruct pv as [pA pv].
+  rewrite (UIP pA eq_refl) in pv. simpl in pv. clear pA.
+  destruct pv. rename v1 into v.
+  apply heq_refl.
+Defined.
+
+Lemma cong_refl :
+  forall (A1 A2 : Type) (u1 : A1) (u2 : A2),
+    A1 ≅ A2 ->
+    u1 ≅ u2 ->
+    @eq_refl A1 u1 ≅ @eq_refl A2 u2.
+Proof.
+  intros A1 A2 u1 u2 pA pu.
+  destruct pA as [pT pA].
+  rewrite (UIP pT eq_refl) in pA. simpl in pA. clear pT.
+  destruct pA. rename A1 into A.
+  destruct pu as [pA pu].
+  rewrite (UIP pA eq_refl) in pu. simpl in pu. clear pA.
+  destruct pu.
+  now apply heq_refl.
+Defined.
+
+Lemma eq_to_heq :
+  forall {A} {u v : A},
+    u = v -> u ≅ v.
+Proof.
+  intros A u v p.
+  exists eq_refl. exact p.
+Defined.
+
+Lemma heq_type_eq :
+  forall {A} {u : A} {B} {v : B},
+    u ≅ v -> A = B.
+Proof.
+  intros A u B v e.
+  now destruct e.
+Defined.
+
+Quote Definition tHeq := @heq.
+Quote Definition tHeqToEq := @heq_to_eq.
+Quote Definition tHeqRefl := @heq_refl.
+Quote Definition tHeqSym := @heq_sym.
+Quote Definition tHeqTrans := @heq_trans.
+Quote Definition tHeqTransport := @heq_transport.
+Quote Definition tPack := @Pack.
+Quote Definition tProjT1 := @ProjT1.
+Quote Definition tProjT2 := @ProjT2.
+Quote Definition tProjTe := @ProjTe.
+Quote Definition tCongProd := @cong_prod.
+Quote Definition tCongLambda := @cong_lambda.
+Quote Definition tCongApp := @cong_app.
+Quote Definition tCongEq := @cong_eq.
+Quote Definition tCongRefl := @cong_refl.
+Quote Definition tEqToHeq := @eq_to_heq.
+Quote Definition tHeqTypeEq := @heq_type_eq.
+
+Definition mkHeq (A a B b : term) : term :=
+  tApp tHeq [ A ; a ; B ; b ].
+
+Definition mkHeqToHeq (A u v p : term) : term :=
+  tApp tHeqToEq [ A ; u ; v ; p ].
+
+Definition mkHeqRefl (A a : term) : term :=
+  tApp tHeqRefl [ A ; a ].
+
+Definition mkHeqSym (A a B b p : term) : term :=
+  tApp tHeqSym [ A ; a ; B ; b ; p ].
+
+Definition mkHeqTrans (A a B b C c p q : term) : term :=
+  tApp tHeqTrans [ A ; a ; B ; b ; C ; c ; p ; q ].
+
+Definition mkHeqTransport (A B p t : term) : term :=
+  tApp tHeqTransport [ A ; B ; p ; t ].
+
+Definition mkPack (A1 A2 : term) : term :=
+  tApp tPack [ A1 ; A2 ].
+
+Definition mkProjT1 (A1 A2 p : term) : term :=
+  tApp tProjT1 [ A1 ; A2 ; p ].
+
+Definition mkProjT2 (A1 A2 p : term) : term :=
+  tApp tProjT2 [ A1 ; A2 ; p ].
+
+Definition mkProjTe (A1 A2 p : term) : term :=
+  tApp tProjTe [ A1 ; A2 ; p ].
+
+Definition mkCongProd (A1 A2 B1 B2 pA pB : term) :=
+  tApp tCongProd [
+    A1 ;
+    A2 ;
+    (tLambda nAnon A1 B1) ;
+    (tLambda nAnon A2 B2) ;
+    pA ;
+    (tLambda nAnon (mkPack A1 A2) pB)
+  ].
+
+Definition mkCongLambda (A1 A2 B1 B2 t1 t2 pA pB pt : term) :=
+  tApp tCongProd [
+    A1 ;
+    A2 ;
+    (tLambda nAnon A1 B1) ;
+    (tLambda nAnon A2 B2) ;
+    (tLambda nAnon A1 t1) ;
+    (tLambda nAnon A2 t2) ;
+    pA ;
+    (tLambda nAnon (mkPack A1 A2) pB) ;
+    (tLambda nAnon (mkPack A1 A2) pt)
+  ].
+
+Definition mkCongApp (A1 A2 B1 B2 t1 t2 u1 u2 pA pB pt pu : term) :=
+  tApp tCongProd [
+    A1 ;
+    A2 ;
+    (tLambda nAnon A1 B1) ;
+    (tLambda nAnon A2 B2) ;
+    t1 ;
+    t2 ;
+    u1 ;
+    u2 ;
+    pA ;
+    (tLambda nAnon (mkPack A1 A2) pB) ;
+    pt ;
+    pu
+  ].
+
+Definition mkCongEq (A1 A2 u1 v1 u2 v2 pA pu pv : term) : term :=
+  tApp tCongEq [ A1 ; A2 ; u1 ; v1 ; u2 ; v2 ; pA ; pu ; pv ].
+
+Definition mkCongRefl (A1 A2 u1 u2 pA pu : term) : term :=
+  tApp tCongRefl [ A1 ; A2 ; u1 ; u2 ; pA ; pu ].
+
+Definition mkEqToHeq (A u v p : term) : term :=
+  tApp tEqToHeq [ A ; u ; v ; p ].
+
+Definition mkHeqTypeEq (A u B v p : term) : term :=
+  tApp tHeqTypeEq [ A ; u ; B ; v ; p ].
